x^2 + 6x + 8 = 0
ax^2 + bx + c = 0
b = 6
c = 8

1 x 8 = 8
2 x 4 = 8

1 + 6 = 8
2 + 4 = 8

(x + 4) (x + 2) = 0

x^2 - 10x + 16 = 0
b = -10
c = 16

1 x 16 = 16
2 x 8 = 16
4x4 = 16

1 + 16 = 17
2 + 8 = 10

(x - 2)(x - 8) = 0

x^2 + 3x - 28
b = 3
c = -28

1 x 28 = 28
2 x 14 = 28
4 x 7 = 28

1 - 28 = 27
2 - 14 = 12
4 - 7 = -3
(x-4)(x+7)
x = 4 and x = 7

x^2 - 64 = 0
x^2 -8x + 8x -64 = 0
x(x-8)+8(x-8) = 0
(x+8)(x-8) = 0

# x^2 + 5x - 14
b = 5
c = -14

1 x -14 = -14
-1 x 14 = -14
2 x -7 = -14
-2 x 7 = 14

2 -7 = -5
-2 + 7 = +5

(x- 2)(x+7)=0
x = 2, x = -7

# x^2 - 169 = 0
(x - 13)(x + 13) = 0
x = 13, x = -13

# x^2 +x - 72 = 0
1 x -72
-1 x 72

2 x -36
-2 x 36

3 x -24
-3 x 24 

4 x -18 
-4 x 18

6 x -12
-6 x 12

8 x -9
-8 x 9
|||||
-8 + 9

(x -8)(x+9) = 0
x = 8, and x = -9

# x^2 + 9x = 0
x(x + 9)
x = 0 and x = -9

# x^2 -3x + 10 = 0
b = -3
c = 10

1 x 10
2 x 5

-1-10 = -11
-2 - 5 = -7
# x^2 -3x - 10 = 0
b = -3
c = -10

-1 x 10
1x -10
2x -5
-2x5

2 - 5 = -3
(x + 2)(x - 5) = 0
x = -2, x = 5










